Finish soundness of dead code decision procedure

src/Language/PlutusIR/Transform/Inline/DecideBool.v
@@ -2,61 +2,146 @@ From Coq Require Import
   String
   List
   Bool
-  Program.
+  Program
+  Utf8_core
+.
 
 From PlutusCert Require Import
   Util
   Language.PlutusIR
   Language.PlutusIR.Analysis.Equality
   Language.PlutusIR.Transform.Congruence
-  Language.PlutusIR.Transform.Let
-  Language.PlutusIR.Transform.Inline.
-
-
-Definition Bindings_desugar' :=
-  fun (Term_desugar : Term -> Term -> bool) =>
-    (fix Bindings_desugar'
-            (bs : list Binding) (t : Term) {struct bs} := match bs with
-            | nil       => Just t
-            | cons b bs => match b, t with
-              | TermBind Strict v rhs, Apply (LamAbs v' _ body') rhs' =>
-                if (String.eqb v v' && Term_desugar rhs rhs')
-                  then Bindings_desugar' bs body'
-                  else None
-                (* Notation scope analysis fails, not sure why....*)
-              | _, _ => None
-              end
-            end).
-
-(*
-  Returns true if the inline transformation was correct
-*)
-Fixpoint dec_inline (env : list (string * Term)) (x y : Term) {struct x} : bool := match x, y with
-  | Var n          , t                  =>
-
-  | Let rec bs t   , Let rec' bs' t'    => Recursivity_eqb rec rec' && list_eqb (dec_inline_Binding env) bs bs' && dec_inline env t t'
-  | TyAbs n k t    , TyAbs n' k' t'     => String.eqb n n' && Kind_eqb k k' && dec_inline env t t'
-  | LamAbs n ty t  , LamAbs n' ty' t'   => String.eqb n n' && Ty_eqb ty ty' && dec_inline env t t'
-  | Apply s t      , Apply s' t'        => dec_inline env s s' && dec_inline env t t'
-  | Constant c     , Constant c'        => some_eqb c c'
-  | Builtin f      , Builtin f'         => func_eqb f f'
-  | TyInst t ty    , TyInst t' ty'      => dec_inline env t t' && Ty_eqb ty ty'
-  | Error ty       , Error ty'          => Ty_eqb ty ty'
-  | IWrap ty1 ty2 t, IWrap ty1' ty2' t' => Ty_eqb ty1 ty1' && Ty_eqb ty2 ty2' && dec_inline env t t'
-  | Unwrap t       , Unwrap t'          => dec_inline env t t'
-
-  | _, _ => false
-  end
-with dec_inline_Binding (env : list (string * Term)) (b b' : Binding) : bool := match b, b' with
-  | TermBind s vdecl t, TermBind s' vdecl' t' => Strictness_eqb s s' && VDecl_eqb vdecl vdecl' && dec_inline env t t'
-  | TypeBind tvdecl ty, TypeBind tvdecl' ty'  => TVDecl_eqb tvdecl tvdecl' && Ty_eqb ty ty'
-  | DatatypeBind dtd  , DatatypeBind dtd'     => DTDecl_eqb dtd dtd'
-  | _, _ => false
-  end
+  Language.PlutusIR.Transform.Inline
 .
 
-(* See comment of Bindings_desugar' *)
-Definition Bindings_desugar
-     : list Binding -> Term -> option Term := Bindings_desugar' Term_desugar.
+Import NamedTerm.
+Import ListNotations.
+
+(* TODO *)
+Axiom some_eqb : some valueOf -> some valueOf -> bool.
+Axiom some_eqb_eq : ∀ x y, some_eqb x y = true -> x = y.
+
+Section Bindings.
+
+  Context (dec_Term : ctx -> Term -> Term -> bool).
+  Context (dec_Term_sound : ∀ Γ s t, dec_Term Γ s t = true -> inline Γ s t).
+  Context (Strictness_eqb_eq : ∀ s s0, Strictness_eqb s s0 = true -> s = s0).
+  Context (VDecl_eqb_eq : ∀ v v0, VDecl_eqb v v0 = true -> v = v0).
+
+  Fixpoint dec_Bindings_Rec (Γ : ctx) (bs bs' : list Binding) : bool := match bs, bs' with
+    | (TermBind s vdecl t :: bs), (TermBind s' vdecl' t' :: bs') =>
+           Strictness_eqb s s'
+        && VDecl_eqb vdecl vdecl'
+        && dec_Term Γ t t'
+        && dec_Bindings_Rec Γ bs bs'
+
+    | (TypeBind tvdecl ty :: bs), (TypeBind tvdecl' ty' :: bs') =>
+           TVDecl_eqb tvdecl tvdecl'
+        && Ty_eqb ty ty'
+        && dec_Bindings_Rec Γ bs bs'
+
+    | (DatatypeBind dtd :: bs) , (DatatypeBind dtd' :: bs')     =>
+          DTDecl_eqb dtd dtd'
+        && dec_Bindings_Rec Γ bs bs'
+
+    | []       , []          => true
+    | _        , _           => false
+    end
+  .
+
+  Set Diffs "on".
+
+  Lemma dec_Bindings_Rec_sound : ∀ Γ bs bs',
+    dec_Bindings_Rec Γ bs bs' = true -> inline_Bindings_Rec Γ bs bs'.
+  Proof with eauto.
+  intros Γ bs.
+  induction bs.
+  all: intros bs' H_true.
+  (* bs = [] *)
+  - destruct bs'.
+    + constructor.
+    + inversion H_true.
+  (* bs = b :: bs*)
+  - destruct bs', a.
+    1, 2, 3: inversion H_true.
+    all: destruct b.
+    + simpl in H_true.
+      repeat (apply andb_true_iff in H_true; destruct H_true as [?H_true ?]).
+      assert (H_v0_v1 : v = v0)...
+      assert (H_s0_s1 : s = s0)...
+      subst.
+      destruct v0.
+      constructor.
+      * eapply inl_TermBind...
+      assert (H_ : v = v0)...
+      assert ()
+      let (H_v_v0 : v0 = v1) _.
+      constructor.
+        *  econstructor.
+
+    + destruct b. 
+      2, 3: inversion H_true.
+      * inversion H_true.
+      * inversion H_true.
+      all: inversion H_true.
+      * inversion H_true.
+    destruct a.
+    + simpl in H_true.
+  simpl in H_true.
+
+  Fixpoint dec_Bindings_NonRec (Γ : ctx) (bs bs' : list Binding) : bool := match bs, bs' with
+    | (b :: bs), (b' :: bs') =>
+        dec_Bindings_NonRec (Binding_to_ctx b ++ Γ) bs bs' &&
+        match b, b' with
+        | (TermBind s vdecl t), (TermBind s' vdecl' t') =>
+             Strictness_eqb s s'
+          && VDecl_eqb vdecl vdecl'
+          && dec_Term Γ t t'
+
+        | (TypeBind tvdecl ty), (TypeBind tvdecl' ty') =>
+           TVDecl_eqb tvdecl tvdecl'
+        && Ty_eqb ty ty'
+
+        | (DatatypeBind dtd) , (DatatypeBind dtd')     =>
+              DTDecl_eqb dtd dtd'
+
+        | _ , _ => false
+        end
+
+    | []       , []          => true
+    | _        , _           => false
+    end
+  .
+
+End Bindings.
+
+Fixpoint dec_Term (Γ : ctx) (x y : Term) {struct x} : bool := match x, y with
+  (*| Var n          , t                  =>*)
+
+  | Var n          , Var m              => String.eqb n m
+
+  | Let NonRec bs t   , Let NonRec bs' t' =>
+      let Γ_bs := Bindings_to_ctx bs in
+         dec_Bindings_NonRec dec_Term Γ bs bs'
+      && dec_Term (Γ ++ Γ_bs) t t'
+
+  | Let Rec bs t   , Let Rec bs' t' =>
+      let Γ_bs := Bindings_to_ctx bs in
+         dec_Bindings_Rec dec_Term (Γ ++ Γ_bs) bs bs'
+      && dec_Term (Γ ++ Γ_bs) t t'
+
+  | TyAbs n k t    , TyAbs n' k' t'     => String.eqb n n' && Kind_eqb k k' && dec_Term Γ t t'
+  | LamAbs n ty t  , LamAbs n' ty' t'   => String.eqb n n' && Ty_eqb ty ty' && dec_Term Γ t t'
+  | Apply s t      , Apply s' t'        => dec_Term Γ s s' && dec_Term Γ t t'
+  | Constant c     , Constant c'        => some_eqb c c'
+  | Builtin f      , Builtin f'         => func_eqb f f'
+  | TyInst t ty    , TyInst t' ty'      => dec_Term Γ t t' && Ty_eqb ty ty'
+  | Error ty       , Error ty'          => Ty_eqb ty ty'
+  | IWrap ty1 ty2 t, IWrap ty1' ty2' t' => Ty_eqb ty1 ty1' && Ty_eqb ty2 ty2' && dec_Term Γ t t'
+  | Unwrap t       , Unwrap t'          => dec_Term Γ t t'
+
+  | _, _ => false
+  end
 
 
+.
